pico-invsubtyping-limitedvpa/ReadonlyProperties.v
@@ -12,7 +12,7 @@ Theorem readonly_pico_field_write :
     (Hstatic_type : static_getType sΓ readonlyx = Some qt)
     (Hqt_ro : sqtype qt = RO)
     (Hwf : wf_r_config CT sΓ rΓ h)
-    (Htyping : stmt_typing CT sΓ stmt sΓ')
+    (Htyping : stmt_typing CT retain_nonabs sΓ stmt sΓ')
     (Heval : eval_stmt OK (reachable_locations_from_initial_env CT h rΓ) true CT rΓ h stmt OK true (reachable_locations_from_initial_env CT h rΓ) rΓ' h')
     (Hget_readonly : runtime_getVal rΓ readonlyx = Some (Iot l))
     (Hobj_before : runtime_getObj h l = Some (mkObj (mkruntime_type anyrq C) vals))
@@ -63,18 +63,18 @@ Proof.
   (* Use the fact that Final/RDA fields are protected from modification *)
   destruct Hassign as [Hfinal | Hrda].
   -  
-    rewrite Hstatic_type in H8.
-    inversion H8.
+    rewrite Hstatic_type in H7.
+    inversion H7.
     subst Tx.
     (* rewrite Hstatic_type in H16. *)
-    unfold vpa_assignability in H17.
+    unfold vpa_assignability in H19.
     destruct a eqn: Haeqn; try easy.
     assert (Hneq: anyf <> f).
     {
       intro Heq.
       subst anyf.
-      unfold sf_assignability_rel in H15, Hfinal.
-      destruct H15 as [fdef_assign [Hlookup_assign Hassign_assign]].
+      unfold sf_assignability_rel in H12, Hfinal.
+      destruct H12 as [fdef_assign [Hlookup_assign Hassign_assign]].
       destruct Hfinal as [fdef_final [Hlookup_final Hassign_final]].
       assert (fdef_final = fdef_assign).
       {
@@ -103,11 +103,11 @@ Proof.
     apply update_diff.
     exact Hneq.
     unfold vpa_assignability in H17.
-    rewrite Hqt_ro in H18; easy.
-    rewrite Hqt_ro in H18; easy.
+    rewrite Hqt_ro in H19; easy.
+    rewrite Hqt_ro in H19; easy.
   - (* RDA case: RDA fields cannot be written *)
-    rewrite Hstatic_type in H8.
-    inversion H8.
+    rewrite Hstatic_type in H7.
+    inversion H7.
     subst Tx.
     unfold vpa_assignability in H17.
     destruct a eqn: Haeqn; try easy.
@@ -115,8 +115,8 @@ Proof.
     {
       intro Heq.
       subst anyf.
-      unfold sf_assignability_rel in H15, Hrda.
-      destruct H15 as [fdef_assign [Hlookup_assign Hassign_assign]].
+      unfold sf_assignability_rel in H12, Hrda.
+      destruct H12 as [fdef_assign [Hlookup_assign Hassign_assign]].
       destruct Hrda as [fdef_final [Hlookup_final Hassign_final]].
       assert (fdef_final = fdef_assign).
       {
@@ -144,13 +144,13 @@ Proof.
     symmetry.
     apply update_diff.
     exact Hneq.
-    rewrite Hqt_ro in H18; easy.
-    rewrite Hqt_ro in H18; easy.
+    rewrite Hqt_ro in H19; easy.
+    rewrite Hqt_ro in H19; easy.
 Qed.
 
 Definition all_params_safe (msig : method_sig) : Prop :=
-  is_safe_mode (sqtype (mreceiver msig)) /\
-  Forall (fun T => is_safe_mode (sqtype T)) (mparams msig).
+  is_safe_mode (mreceiver msig) /\
+  Forall (fun T => is_safe_mode T) (mparams msig).
 
 Definition protected_locations_from_vals
   (CT : class_table) (h : heap) (vals : list value) : Ensembles.Ensemble Loc :=
@@ -208,14 +208,14 @@ Proof.
 Qed.
 
 Theorem readonly_method_call_preserves_arguments :
-  forall CT sΓ rΓ h stmt rΓ' h' sΓ' x y mindex Ty mdef zs anyC vals ly 
+  forall CT sΓ rΓ h stmt rΓ' h' sΓ' x y mindex Ty mdef zs anyabs anyC vals ly 
          loc_arg C anyrq vals_arg vals_arg' f
     (Hstmt : stmt = (SCall x mindex y zs))
-    (HTy : Ty = Build_qualified_type RO anyC)
+    (HTy : Ty = Build_qualified_type anyabs RO anyC)
     (Hstatic_type : static_getType sΓ y = Some Ty)
     (Hmethod_lookup : FindMethodWithName CT (sctype Ty) mindex mdef)
     (Hwf : wf_r_config CT sΓ rΓ h)
-    (Htyping : stmt_typing CT sΓ stmt sΓ')
+    (Htyping : stmt_typing CT retain_nonabs sΓ stmt sΓ')
     (Heval : eval_stmt OK (reachable_locations_from_initial_env CT h rΓ) true CT rΓ h stmt OK true (reachable_locations_from_initial_env CT h rΓ) rΓ' h')
     (Hget_y : runtime_getVal rΓ y = Some (Iot ly))
     (Hget_zs : runtime_lookup_list rΓ zs = Some vals)
@@ -243,7 +243,7 @@ Proof.
   subst vals0.
   inversion Htyping; subst.
   rename sΓ' into sΓ.
-  have HTy: Ty = {| sqtype := RO; sctype := anyC |}.
+  have HTy: Ty = {| sabs := anyabs; sqtype := RO; sctype := anyC |}.
   {
     rewrite H12 in Hstatic_type.
     inversion Hstatic_type.
@@ -362,7 +362,7 @@ Proof.
         rewrite HeqrΓmethodinit.
         simpl.
         f_equal.
-        apply Forall2_length in H23.
+        apply Forall2_length in H24.
         assert (Hy_dom : y < dom sΓ).
         {
           apply static_getType_dom in H12.
@@ -408,7 +408,7 @@ Proof.
         }
         rewrite H1.
         rewrite H5.
-        rewrite <- H23.
+        rewrite <- H24.
         exact H13.
 
         (* Correspondence holds for inner environment *)
@@ -477,14 +477,14 @@ Proof.
 
         (* Base type subtyping *)
         rewrite Hmsigeq.
-        apply qualified_type_subtype_base_subtype in H22.
-        rewrite (vpa_mutabilty_tt_sctype Ty (mreceiver (msignature mdef1))) in H22.
+        apply qualified_type_subtype_base_subtype in H23.
+        rewrite (vpa_mutabilty_tt_sctype Ty (mreceiver (msignature mdef1))) in H23.
         eapply base_trans; eauto.
 
         (* Qualifier typbility *)
         1: 
         {
-          apply qualified_type_subtype_q_subtype in H22.
+          apply qualified_type_subtype_q_subtype in H23.
           specialize (Hcorrcopy lOutterReceiver OutterReceiverMutability HOutterReceiverAddr HOutterReceiverMutabilityType).
           apply get_this_qualified_type_nth_error in H14.
           unfold wf_senv in Hsenv.
@@ -539,8 +539,8 @@ Proof.
           unfold vpa_mutabilty_rs.
           unfold vpa_mutabilty_rs in HyQualifierTypablility.
           unfold vpa_mutabilty_rs in Houtter_qualifier_typable.
-          unfold vpa_mutabilty_tt in H22.
-          rewrite <- Hmsigeq in H22.
+          unfold vpa_mutabilty_tt in H23.
+          rewrite <- Hmsigeq in H23.
 
           destruct qinner eqn:HInnerReceiverMutability;
           destruct (sqtype (mreceiver (msignature mdef))) eqn:HMethodReceiverDeclaredType;
@@ -549,11 +549,11 @@ Proof.
           destruct (sqtype Ty) eqn:HTyStaticMutability;
           try trivial.
           all: destruct (sqtype Tthis) eqn:HTthisStaticMutability;
-          try rewrite HTyStaticMutability in H22;
-          simpl in H22;
-          try rewrite HMethodReceiverDeclaredType in H22;
-          try inversion H22; try trivial.
-          all: try inversion H22; try easy.
+          try rewrite HTyStaticMutability in H23;
+          simpl in H23;
+          try rewrite HMethodReceiverDeclaredType in H23;
+          try inversion H23; try trivial.
+          all: try inversion H23; try easy.
         }
 
         (* -------------------------------------------------- *)
@@ -567,11 +567,11 @@ Proof.
             (* Use H23 to get the subtyping relationship *)
             assert (Hi'_bound : i' < List.length argtypes).
             {
-              apply Forall2_length in H23.
+              apply Forall2_length in H24.
               simpl in Hi.
               simpl in Hnth.
               rewrite Hmsigeq in Hnth.
-              rewrite H23.
+              rewrite H24.
               apply nth_error_Some.
               intros Hnone.
               rewrite Hnth in Hnone.
@@ -657,16 +657,16 @@ Proof.
             (* base subtype *)
             rewrite nth_error_cons_succ in Hnth.
             rewrite Hmsigeq in Hnth.
-            eapply Forall2_nth_error in H23; eauto.
-            apply qualified_type_subtype_base_subtype in H23.
-            rewrite (vpa_mutabilty_tt_sctype Ty sqt) in H23.
+            eapply Forall2_nth_error in H24; eauto.
+            apply qualified_type_subtype_base_subtype in H24.
+            rewrite (vpa_mutabilty_tt_sctype Ty sqt) in H24.
             eapply base_trans; eauto.
 
             (* Qualifier Typability *)
             rewrite Hmsigeq in Hnth.
-            eapply Forall2_nth_error in H23; eauto.
-            apply qualified_type_subtype_q_subtype in H23.
-            rewrite sq_vpa_tt_eq_qq in H23.
+            eapply Forall2_nth_error in H24; eauto.
+            apply qualified_type_subtype_q_subtype in H24.
+            rewrite sq_vpa_tt_eq_qq in H24.
             specialize (Hcorrcopy_2 lOutterReceiver OutterReceiverMutability HOutterReceiverAddr HOutterReceiverMutabilityType).
             unfold wf_senv in Hsenv.
             destruct Hsenv as [Hsenvdom _].
@@ -709,7 +709,7 @@ Proof.
               easy.
             }
             subst rq_obj.
-            clear - H23 Harg_qualifiertypability HyQualifierTypablility HOutterReceiverQualifierTypablility Ty.
+            clear - H24 Harg_qualifiertypability HyQualifierTypablility HOutterReceiverQualifierTypablility Ty.
 
             destruct (rqtype (rt_type argobj)) eqn:Hargobjmutability; move Hargobjmutability at bottom;
             destruct (sqtype sqt) eqn:HParameterStaticDeclearedMutability; move HParameterStaticDeclearedMutability at bottom;
@@ -718,7 +718,7 @@ Proof.
 
             all: destruct (sqtype Ty) eqn:HTyStaticMutability;
             destruct (sqtype argtype) eqn:HArgTypeStaticMutability;
-            simpl in H23;
+            simpl in H24;
             try solve_q_subtype_wrong.
 
             all: 
@@ -730,10 +730,10 @@ Proof.
             apply nth_error_None in Hval_i.
             apply runtime_lookup_list_preserves_length in H5.
             apply static_getType_list_preserves_length in H13.
-            apply Forall2_length in H23.
+            apply Forall2_length in H24.
             rewrite H5 in Hval_i.
             rewrite <- H13 in Hval_i.
-            rewrite H23 in Hval_i.
+            rewrite H24 in Hval_i.
             simpl in Hi.
             simpl in Hnth.
             rewrite <- Hmsigeq in Hval_i.
@@ -741,7 +741,56 @@ Proof.
     }
     rewrite getmbody in H7.
     have HtrueVal: TouchNonMutOnly = true.
-    eapply eval_stmt_did_not_touch_abs_start_with_true; eauto.
+    (* rewrite getmbody in Heval. *)
+    eapply eval_stmt_did_not_touch_abs_start_with_true with (P:=(reachable_locations_from_initial_env CT h rΓmethodinit)) (rΓ':=rΓ'')(h':=h'); eauto.
+    assert (Hy_dom : y < dom sΓ).
+    {
+      apply static_getType_dom in H12.
+      exact H12.
+    }
+    assert (HOutterReceiverAddr: exists lOutterReceiver, get_this_var_mapping (vars rΓ) = Some lOutterReceiver).
+    {
+      eapply get_this_exists_from_wf_r_config; eauto.
+    }
+    destruct HOutterReceiverAddr as [lOutterReceiver HOutterReceiverAddr].
+    assert (HOutterReceiverMutability: exists qcontext, r_muttype h lOutterReceiver = Some qcontext).
+    {
+      eapply receiver_mutability_exists_wf_renv; eauto.
+    }
+    destruct HOutterReceiverMutability as [OutterReceiverMutability HOutterReceiverMutabilityType].
+    have Hcorr := Htypable.
+    have Hcorrcopy := Hcorr.
+    specialize (Hcorr lOutterReceiver OutterReceiverMutability HOutterReceiverAddr HOutterReceiverMutabilityType y Hy_dom Ty H12).
+    unfold wf_r_typable in Hcorr.
+    unfold r_basetype in H1.
+    unfold r_type.
+    destruct (runtime_getObj h ly) as [obj|] eqn:Hobjy; [|discriminate].
+    injection H1 as Hcy_eq.
+    subst cy.
+    destruct obj as [rt_obj fields_obj].
+    destruct rt_obj as [rq_obj rc_obj].
+
+    have Hrenvcopy := Hrenv.
+    unfold wf_renv in Hrenv.
+    destruct Hrenv as [_ [Hreceiver _]].
+    destruct Hreceiver as [iot [Hget_iot _]].
+    unfold get_this_var_mapping.
+    unfold gget in Hget_iot.
+    destruct (vars rΓ) as [|v0 vs] eqn:Hvars; [discriminate|].
+
+    unfold r_type in Hcorr.
+    rewrite H0 in Hcorr.
+    rewrite Hobjy in Hcorr.
+    simpl in Hcorr.
+    destruct Hcorr as [Hbasesubtype HyQualifierTypablility].
+    
+    assert (Hmsigeq: msignature mdef = msignature mdef1).
+    {
+      eapply method_signature_consistent_subtype; eauto.
+    }
+    rewrite <- Hmsigeq in H17.
+    rewrite H17 in Hmethodbody_typing.
+    exact Hmethodbody_typing.
     subst TouchNonMutOnly.
     eapply deep_readonly_preservation with (stmt := (mbody_stmt mbody)) (sΓ' := sΓmethodend) (rΓ' := rΓ''); eauto.
     assert (HenvImpliesEnvRespect: env_respects_protected_set (reachable_locations_from_initial_env CT h rΓmethodinit) sΓmethodinit rΓmethodinit).
@@ -811,8 +860,53 @@ Proof.
         eapply Forall_nth_error in Hall_params; eauto.
     }
     exact HenvImpliesEnvRespect.
-    rewrite getmbody; exact Hmethodbody_typing.
-    rewrite getmbody; auto.
+    assert (Hy_dom : y < dom sΓ).
+    {
+      apply static_getType_dom in H12.
+      exact H12.
+    }
+    assert (HOutterReceiverAddr: exists lOutterReceiver, get_this_var_mapping (vars rΓ) = Some lOutterReceiver).
+    {
+      eapply get_this_exists_from_wf_r_config; eauto.
+    }
+    destruct HOutterReceiverAddr as [lOutterReceiver HOutterReceiverAddr].
+    assert (HOutterReceiverMutability: exists qcontext, r_muttype h lOutterReceiver = Some qcontext).
+    {
+      eapply receiver_mutability_exists_wf_renv; eauto.
+    }
+    destruct HOutterReceiverMutability as [OutterReceiverMutability HOutterReceiverMutabilityType].
+    have Hcorr := Htypable.
+    have Hcorrcopy := Hcorr.
+    specialize (Hcorr lOutterReceiver OutterReceiverMutability HOutterReceiverAddr HOutterReceiverMutabilityType y Hy_dom Ty H12).
+    unfold wf_r_typable in Hcorr.
+    unfold r_basetype in H1.
+    unfold r_type.
+    destruct (runtime_getObj h ly) as [obj|] eqn:Hobjy; [|discriminate].
+    injection H1 as Hcy_eq.
+    subst cy.
+    destruct obj as [rt_obj fields_obj].
+    destruct rt_obj as [rq_obj rc_obj].
+
+    unfold wf_renv in Hrenv.
+    destruct Hrenv as [_ [Hreceiver _]].
+    destruct Hreceiver as [iot [Hget_iot _]].
+    unfold get_this_var_mapping.
+    unfold gget in Hget_iot.
+    destruct (vars rΓ) as [|v0 vs] eqn:Hvars; [discriminate|].
+
+    unfold r_type in Hcorr.
+    rewrite H0 in Hcorr.
+    rewrite Hobjy in Hcorr.
+    simpl in Hcorr.
+    destruct Hcorr as [Hbasesubtype HyQualifierTypablility].
+    assert (Hmsigeq: msignature mdef = msignature mdef1).
+    {
+      eapply method_signature_consistent_subtype; eauto.
+    }
+    rewrite getmbody. rewrite <- Hmsigeq in H17.
+    rewrite H17 in Hmethodbody_typing.
+    exact Hmethodbody_typing.
+    rewrite getmbody. auto.
     have Hsubset := protected_locations_subset_reachable_from_method_frame CT h ly vals.
     rewrite <- HeqrΓmethodinit in Hsubset.
     unfold Ensembles.Included in Hsubset.
@@ -832,7 +926,7 @@ Proof.
     remember (mreceiver (msignature mdef) :: mparams (msignature mdef)) as sΓmethodinit;
     remember {| vars := Iot ly :: vals |} as rΓmethodinit;
     remember (rΓ <| vars := update x retval (vars rΓ) |>) as rΓ'''.
-    remember {| sqtype := RO; sctype := anyC |} as Ty. 
+    remember {| sabs := anyabs; sqtype := RO; sctype := anyC |} as Ty. 
     assert(Hwf_method_frame : wf_r_config CT sΓmethodinit rΓmethodinit h).
     {
       (* Method inner config wellformed.*)
@@ -918,7 +1012,7 @@ Proof.
         rewrite HeqrΓmethodinit.
         simpl.
         f_equal.
-        apply Forall2_length in H23.
+        apply Forall2_length in H24.
         assert (Hy_dom : y < dom sΓ).
         {
           apply static_getType_dom in H12.
@@ -965,7 +1059,7 @@ Proof.
         }
         rewrite H1.
         rewrite H5.
-        rewrite <- H23.
+        rewrite <- H24.
         exact H13.
 
         (* Correspondence holds for inner environment *)
@@ -1034,15 +1128,15 @@ Proof.
 
         (* Base type subtyping *)
         rewrite Hmsigeq.
-        apply qualified_type_subtype_base_subtype in H22.
+        apply qualified_type_subtype_base_subtype in H23.
         (* rewrite (vpa_mutabilty_tt_sctype Tthis Ty) in H23. *)
-        rewrite (vpa_mutabilty_tt_sctype Ty (mreceiver (msignature mdef1))) in H22.
+        rewrite (vpa_mutabilty_tt_sctype Ty (mreceiver (msignature mdef1))) in H23.
         eapply base_trans; eauto.
 
         (* Qualifier typbility *)
         1: 
         {
-          apply qualified_type_subtype_q_subtype in H22.
+          apply qualified_type_subtype_q_subtype in H23.
           specialize (Hcorrcopy lOutterReceiver OutterReceiverMutability HOutterReceiverAddr HOutterReceiverMutabilityType).
           apply get_this_qualified_type_nth_error in H14.
           unfold wf_senv in Hsenv.
@@ -1097,8 +1191,8 @@ Proof.
           unfold vpa_mutabilty_rs.
           unfold vpa_mutabilty_rs in HyQualifierTypablility.
           unfold vpa_mutabilty_rs in Houtter_qualifier_typable.
-          unfold vpa_mutabilty_tt in H22.
-          rewrite <- Hmsigeq in H22.
+          unfold vpa_mutabilty_tt in H23.
+          rewrite <- Hmsigeq in H23.
 
           destruct qinner eqn:HInnerReceiverMutability;
           destruct (sqtype (mreceiver (msignature mdef))) eqn:HMethodReceiverDeclaredType;
@@ -1107,11 +1201,11 @@ Proof.
           destruct (sqtype Ty) eqn:HTyStaticMutability;
           try trivial.
           all: destruct (sqtype Tthis) eqn:HTthisStaticMutability;
-          try rewrite HTyStaticMutability in H22;
-          simpl in H22;
-          try rewrite HMethodReceiverDeclaredType in H22;
-          try inversion H22; try trivial.
-          all: try inversion H22; try easy.
+          try rewrite HTyStaticMutability in H23;
+          simpl in H23;
+          try rewrite HMethodReceiverDeclaredType in H23;
+          try inversion H23; try trivial.
+          all: try inversion H23; try easy.
         }
         (* clear_dups. amazing.... *)
 
@@ -1126,11 +1220,11 @@ Proof.
             (* Use H23 to get the subtyping relationship *)
             assert (Hi'_bound : i' < List.length argtypes).
             {
-              apply Forall2_length in H23.
+              apply Forall2_length in H24.
               simpl in Hi.
               simpl in Hnth.
               rewrite Hmsigeq in Hnth.
-              rewrite H23.
+              rewrite H24.
               apply nth_error_Some.
               intros Hnone.
               rewrite Hnth in Hnone.
@@ -1216,16 +1310,16 @@ Proof.
             (* base subtype *)
             rewrite nth_error_cons_succ in Hnth.
             rewrite Hmsigeq in Hnth.
-            eapply Forall2_nth_error in H23; eauto.
-            apply qualified_type_subtype_base_subtype in H23.
-            rewrite (vpa_mutabilty_tt_sctype Ty sqt) in H23.
+            eapply Forall2_nth_error in H24; eauto.
+            apply qualified_type_subtype_base_subtype in H24.
+            rewrite (vpa_mutabilty_tt_sctype Ty sqt) in H24.
             eapply base_trans; eauto.
 
             (* Qualifier Typability *)
             rewrite Hmsigeq in Hnth.
-            eapply Forall2_nth_error in H23; eauto.
-            apply qualified_type_subtype_q_subtype in H23.
-            rewrite sq_vpa_tt_eq_qq in H23.
+            eapply Forall2_nth_error in H24; eauto.
+            apply qualified_type_subtype_q_subtype in H24.
+            rewrite sq_vpa_tt_eq_qq in H24.
             specialize (Hcorrcopy_2 lOutterReceiver OutterReceiverMutability HOutterReceiverAddr HOutterReceiverMutabilityType).
             unfold wf_senv in Hsenv.
             destruct Hsenv as [Hsenvdom _].
@@ -1268,7 +1362,7 @@ Proof.
               easy.
             }
             subst rq_obj.
-            clear - H23 Harg_qualifiertypability HyQualifierTypablility HOutterReceiverQualifierTypablility.
+            clear - H24 Harg_qualifiertypability HyQualifierTypablility HOutterReceiverQualifierTypablility.
 
             destruct (rqtype (rt_type argobj)) eqn:Hargobjmutability; move Hargobjmutability at bottom;
             destruct (sqtype sqt) eqn:HParameterStaticDeclearedMutability; move HParameterStaticDeclearedMutability at bottom;
@@ -1277,7 +1371,7 @@ Proof.
 
             all: destruct (sqtype Ty) eqn:HTyStaticMutability;
             destruct (sqtype argtype) eqn:HArgTypeStaticMutability;
-            simpl in H23;
+            simpl in H24;
             try solve_q_subtype_wrong.
 
             all: 
@@ -1289,10 +1383,10 @@ Proof.
             apply nth_error_None in Hval_i.
             apply runtime_lookup_list_preserves_length in H5.
             apply static_getType_list_preserves_length in H13.
-            apply Forall2_length in H23.
+            apply Forall2_length in H24.
             rewrite H5 in Hval_i.
             rewrite <- H13 in Hval_i.
-            rewrite H23 in Hval_i.
+            rewrite H24 in Hval_i.
             simpl in Hi.
             simpl in Hnth.
             rewrite <- Hmsigeq in Hval_i.
@@ -1300,7 +1394,55 @@ Proof.
     }
     rewrite getmbody in H7.
     have HtrueVal: TouchNonMutOnly = true.
-    eapply eval_stmt_did_not_touch_abs_start_with_true; eauto.
+    eapply eval_stmt_did_not_touch_abs_start_with_true with (P:=(reachable_locations_from_initial_env CT h rΓmethodinit)) (rΓ':=rΓ'')(h':=h'); eauto.
+    assert (Hy_dom : y < dom sΓ).
+    {
+      apply static_getType_dom in H12.
+      exact H12.
+    }
+    assert (HOutterReceiverAddr: exists lOutterReceiver, get_this_var_mapping (vars rΓ) = Some lOutterReceiver).
+    {
+      eapply get_this_exists_from_wf_r_config; eauto.
+    }
+    destruct HOutterReceiverAddr as [lOutterReceiver HOutterReceiverAddr].
+    assert (HOutterReceiverMutability: exists qcontext, r_muttype h lOutterReceiver = Some qcontext).
+    {
+      eapply receiver_mutability_exists_wf_renv; eauto.
+    }
+    destruct HOutterReceiverMutability as [OutterReceiverMutability HOutterReceiverMutabilityType].
+    have Hcorr := Htypable.
+    have Hcorrcopy := Hcorr.
+    specialize (Hcorr lOutterReceiver OutterReceiverMutability HOutterReceiverAddr HOutterReceiverMutabilityType y Hy_dom Ty H12).
+    unfold wf_r_typable in Hcorr.
+    unfold r_basetype in H1.
+    unfold r_type.
+    destruct (runtime_getObj h ly) as [obj|] eqn:Hobjy; [|discriminate].
+    injection H1 as Hcy_eq.
+    subst cy.
+    destruct obj as [rt_obj fields_obj].
+    destruct rt_obj as [rq_obj rc_obj].
+
+    have Hrenvcopy := Hrenv.
+    unfold wf_renv in Hrenv.
+    destruct Hrenv as [_ [Hreceiver _]].
+    destruct Hreceiver as [iot [Hget_iot _]].
+    unfold get_this_var_mapping.
+    unfold gget in Hget_iot.
+    destruct (vars rΓ) as [|v0 vs] eqn:Hvars; [discriminate|].
+
+    unfold r_type in Hcorr.
+    rewrite H0 in Hcorr.
+    rewrite Hobjy in Hcorr.
+    simpl in Hcorr.
+    destruct Hcorr as [Hbasesubtype HyQualifierTypablility].
+    
+    assert (Hmsigeq: msignature mdef = msignature mdef1).
+    {
+      eapply method_signature_consistent_subtype; eauto.
+    }
+    rewrite <- Hmsigeq in H17.
+    rewrite H17 in Hmethodbody_typing.
+    exact Hmethodbody_typing.
     subst TouchNonMutOnly.
     eapply deep_readonly_preservation with (stmt := (mbody_stmt mbody)) (sΓ' := sΓmethodend)(rΓ':=rΓ''); eauto.
     assert (HenvImpliesEnvRespect: env_respects_protected_set (reachable_locations_from_initial_env CT h rΓmethodinit) sΓmethodinit rΓmethodinit).
@@ -1370,7 +1512,52 @@ Proof.
         eapply Forall_nth_error in Hall_params; eauto.
     }
     exact HenvImpliesEnvRespect.
-    rewrite getmbody; exact Hmethodbody_typing.
+    assert (Hy_dom : y < dom sΓ).
+    {
+      apply static_getType_dom in H12.
+      exact H12.
+    }
+    assert (HOutterReceiverAddr: exists lOutterReceiver, get_this_var_mapping (vars rΓ) = Some lOutterReceiver).
+    {
+      eapply get_this_exists_from_wf_r_config; eauto.
+    }
+    destruct HOutterReceiverAddr as [lOutterReceiver HOutterReceiverAddr].
+    assert (HOutterReceiverMutability: exists qcontext, r_muttype h lOutterReceiver = Some qcontext).
+    {
+      eapply receiver_mutability_exists_wf_renv; eauto.
+    }
+    destruct HOutterReceiverMutability as [OutterReceiverMutability HOutterReceiverMutabilityType].
+    have Hcorr := Htypable.
+    have Hcorrcopy := Hcorr.
+    specialize (Hcorr lOutterReceiver OutterReceiverMutability HOutterReceiverAddr HOutterReceiverMutabilityType y Hy_dom Ty H12).
+    unfold wf_r_typable in Hcorr.
+    unfold r_basetype in H1.
+    unfold r_type.
+    destruct (runtime_getObj h ly) as [obj|] eqn:Hobjy; [|discriminate].
+    injection H1 as Hcy_eq.
+    subst cy.
+    destruct obj as [rt_obj fields_obj].
+    destruct rt_obj as [rq_obj rc_obj].
+
+    unfold wf_renv in Hrenv.
+    destruct Hrenv as [_ [Hreceiver _]].
+    destruct Hreceiver as [iot [Hget_iot _]].
+    unfold get_this_var_mapping.
+    unfold gget in Hget_iot.
+    destruct (vars rΓ) as [|v0 vs] eqn:Hvars; [discriminate|].
+
+    unfold r_type in Hcorr.
+    rewrite H0 in Hcorr.
+    rewrite Hobjy in Hcorr.
+    simpl in Hcorr.
+    destruct Hcorr as [Hbasesubtype HyQualifierTypablility].
+    assert (Hmsigeq: msignature mdef = msignature mdef1).
+    {
+      eapply method_signature_consistent_subtype; eauto.
+    }
+    rewrite getmbody. rewrite <- Hmsigeq in H17.
+    rewrite H17 in Hmethodbody_typing.
+    exact Hmethodbody_typing.
     rewrite getmbody; auto.
     have Hsubset := protected_locations_subset_reachable_from_method_frame CT h ly vals.
     rewrite <- HeqrΓmethodinit in Hsubset.
