pico-invsubtyping-limitedvpa/WFNOMutationEXP.v
@@ -7,9 +7,9 @@ Require Import Properties DeepImmutability Reachability.
 Require Import ReadonlyReachability.
 
 Theorem well_typed_no_mutation_exp :
-  forall CT sΓ rΓ h x f y sΓ' loc_x o a vf val_y
+  forall CT mt sΓ rΓ h x f y sΓ' loc_x o a vf val_y
     (Hwf : wf_r_config CT sΓ rΓ h)
-    (Htyping : stmt_typing CT sΓ (SFldWrite x f y) sΓ')
+    (Htyping : stmt_typing CT mt sΓ (SFldWrite x f y) sΓ')
     (Hgetval_x : runtime_getVal rΓ x = Some (Iot loc_x))
     (Hgetobj : runtime_getObj h loc_x = Some o)
     (Hgetval_f : getVal o.(fields_map) f = Some vf)
@@ -20,6 +20,58 @@ Theorem well_typed_no_mutation_exp :
 Proof.
   intros.
   inversion Htyping; subst.
+  rename sΓ' into sΓ.
+  destruct (extract_receiver_from_wf_config CT sΓ rΓ h Hwf) as [iot [qcontext [Hget_iot[Hiot_dom Hqcontext]]]].
+  unfold wf_r_config in Hwf.
+  destruct Hwf as [Hclass [Hheap [Hrenv [Hsenv [Hlen Hcorr]]]]].
+  specialize (Hcorr iot qcontext Hget_iot Hqcontext).
+  have Hxdom: x < dom sΓ by (apply static_getType_dom in H3; auto).
+  specialize (Hcorr x Hxdom Tx H3).
+  rewrite Hgetval_x in Hcorr.
+  unfold wf_r_typable in Hcorr.
+  unfold r_type in Hcorr.
+  rewrite Hgetobj in Hcorr.
+  destruct Hcorr as [Hbase Hqualifer].
+  assert (sf_assignability_rel CT (rctype (rt_type o)) f a0).
+  {
+    eapply sf_assignability_subtyping; eauto.
+  }
+  assert (a0 = a).
+  {
+    eapply sf_assignability_deterministic_rel; eauto.
+  }
+  subst a0.
+  unfold runtime_vpa_assignability in Hvpa_final.
+  unfold vpa_assignability in H12.
+  destruct a eqn: Heq_a; destruct (rqtype (rt_type o)) eqn: Heq_rq;
+  destruct (sqtype Tx) eqn: Heq_sq; try discriminate.
+  destruct qcontext eqn: Heq_qc; try easy.
+  rename sΓ' into sΓ.
+  destruct (extract_receiver_from_wf_config CT sΓ rΓ h Hwf) as [iot [qcontext [Hget_iot[Hiot_dom Hqcontext]]]].
+  unfold wf_r_config in Hwf.
+  destruct Hwf as [Hclass [Hheap [Hrenv [Hsenv [Hlen Hcorr]]]]].
+  specialize (Hcorr iot qcontext Hget_iot Hqcontext).
+  have Hxdom: x < dom sΓ by (apply static_getType_dom in H3; auto).
+  specialize (Hcorr x Hxdom Tx H3).
+  rewrite Hgetval_x in Hcorr.
+  unfold wf_r_typable in Hcorr.
+  unfold r_type in Hcorr.
+  rewrite Hgetobj in Hcorr.
+  destruct Hcorr as [Hbase Hqualifer].
+  assert (sf_assignability_rel CT (rctype (rt_type o)) f a0).
+  {
+    eapply sf_assignability_subtyping; eauto.
+  }
+  assert (a0 = a).
+  {
+    eapply sf_assignability_deterministic_rel; eauto.
+  }
+  subst a0.
+  unfold runtime_vpa_assignability in Hvpa_final.
+  unfold vpa_assignability in H14.
+  destruct a eqn: Heq_a; destruct (rqtype (rt_type o)) eqn: Heq_rq;
+  destruct (sqtype Tx) eqn: Heq_sq; try discriminate.
+  destruct qcontext eqn: Heq_qc; try easy.
   rename sΓ' into sΓ.
   destruct (extract_receiver_from_wf_config CT sΓ rΓ h Hwf) as [iot [qcontext [Hget_iot[Hiot_dom Hqcontext]]]].
   unfold wf_r_config in Hwf.
